{
 "cells": [
  {
   "cell_type": "markdown",
   "metadata": {
    "slideshow": {
     "slide_type": "slide"
    }
   },
   "source": [
    "# Chapter 9: Infinite Series"
   ]
  },
  {
   "cell_type": "markdown",
   "metadata": {
    "slideshow": {
     "slide_type": "slide"
    }
   },
   "source": [
    "### Section 9.9: Representation of Functions by Power Series\n",
    "\n",
    "### Section Objectives:\n",
    "##### Objective 1: Find a geometric power series that represents a function\n",
    "##### Objective 2: Construct a power series using series operations"
   ]
  },
  {
   "cell_type": "markdown",
   "metadata": {
    "slideshow": {
     "slide_type": "slide"
    }
   },
   "source": [
    "##### Objective 1: Find a geometric power series that represents a function"
   ]
  },
  {
   "cell_type": "markdown",
   "metadata": {
    "slideshow": {
     "slide_type": "fragment"
    }
   },
   "source": [
    "##### Review of Geometric Series\n",
    "\n",
    "* Recall that a geometric series is a series of the form\n",
    "\n",
    "\\begin{align}\n",
    "    \\sum_{k = 0}^{\\infty} a_0 r^k\n",
    "\\end{align}\n",
    "\n",
    "* Recall, also, that the sum of a convergent geometric series ($|r| < 1$) is determined by\n",
    "\n",
    "\\begin{align}\n",
    "    \\sum_{k = 0}^{\\infty} a_0 r^k = S = \\frac{a_0}{1 - r}\n",
    "\\end{align}"
   ]
  },
  {
   "cell_type": "markdown",
   "metadata": {
    "slideshow": {
     "slide_type": "fragment"
    }
   },
   "source": [
    "##### Functions Represented as Power Series\n",
    "\n",
    "* Suppose we define a geometric series with $a_0 = 1$ and $r = x$, where $x$ is a real number such that $|x| < 1$\n",
    "\n",
    "* Then we would have a geometric series that is in the form of a power series:\n",
    "\n",
    "\\begin{align}\n",
    "    f(x) & = \\sum_{k = 0}^\\infty x^k\n",
    "\\end{align}\n",
    "\n",
    "* Furthermore, since $S = \\frac{a_0}{1 - r}$ with $a_0 = 1$ and $r = x$ such that $|r| = |x| < 1$ we have $f(x) = \\frac{1}{1 - x}$\n",
    "\n",
    "* The interval of convergence is $(-1, 1)$ since the series diverges for $|r| = |x| \\geq 1$\n",
    "\n",
    "* In fact, we can express any function of the form $f(x) = \\frac{a}{b - cx}$ with nonzero constants $a, b,$ and $c$ as a power series, provided $\\left| \\frac{c x}{b} \\right| < 1$ with interval of convergence to be determined"
   ]
  },
  {
   "cell_type": "markdown",
   "metadata": {
    "slideshow": {
     "slide_type": "fragment"
    }
   },
   "source": [
    "##### Example 1\n",
    "\n",
    "Find a power series for $f(x) = \\frac{4}{x + 2}$, centered at $c = 0$."
   ]
  },
  {
   "cell_type": "markdown",
   "metadata": {
    "slideshow": {
     "slide_type": "fragment"
    }
   },
   "source": [
    "* We rewrite the function:\n",
    "\n",
    "\\begin{align}\n",
    "    f(x) & = \\frac{4}{x + 2} \\\\\n",
    "    & = \\frac{4}{2 + x} \\\\\n",
    "    & = \\frac{4}{2 - (-x)} \\\\\n",
    "    & = \\frac{4}{2 \\left( 1 - \\left( -\\frac{x}{2} \\right) \\right)} \\\\\n",
    "    & = \\frac{\\frac{4}{2}}{1 - \\left( -\\frac{x}{2} \\right)} \\\\\n",
    "    & = \\frac{2}{1 - \\left( -\\frac{x}{2} \\right)} \\\\\n",
    "\\end{align}"
   ]
  },
  {
   "cell_type": "markdown",
   "metadata": {
    "slideshow": {
     "slide_type": "fragment"
    }
   },
   "source": [
    "* This can be seen as a geometric series with $a_0 = 2$ and $r = -\\frac{x}{2}$"
   ]
  },
  {
   "cell_type": "markdown",
   "metadata": {
    "slideshow": {
     "slide_type": "fragment"
    }
   },
   "source": [
    "* Therefore, we can express the function as a power series in the form\n",
    "\n",
    "\\begin{align}\n",
    "    f(x) & = \\sum_{k = 0}^\\infty 2 \\left( - \\frac{x}{2} \\right)^k \\\\\n",
    "    & = \\sum_{k = 0}^\\infty 2 \\left( - \\frac{1}{2} \\right)^k x^k \n",
    "\\end{align}"
   ]
  },
  {
   "cell_type": "markdown",
   "metadata": {
    "slideshow": {
     "slide_type": "fragment"
    }
   },
   "source": [
    "* The interval of convergence is determined by $|r| = \\left| -\\frac{x}{2} \\right| < 1$"
   ]
  },
  {
   "cell_type": "markdown",
   "metadata": {
    "slideshow": {
     "slide_type": "fragment"
    }
   },
   "source": [
    "* Therefore, the interval of convergence is\n",
    "\n",
    "\\begin{align}\n",
    "    & \\left| - \\frac{x}{2} \\right| = \\left| \\frac{x}{2} \\right| < 1 \\\\\n",
    "    & \\Rightarrow |x| < 2 \\\\\n",
    "    & \\Rightarrow -2 < x < 2\n",
    "\\end{align}\n",
    "\n",
    "* Or in interval notation: $(-2, 2)$"
   ]
  },
  {
   "cell_type": "markdown",
   "metadata": {
    "slideshow": {
     "slide_type": "fragment"
    }
   },
   "source": [
    "##### Example 2 \n",
    "\n",
    "Find a power series for $f(x) = \\frac{1}{x}$, centered at $c = 1$."
   ]
  },
  {
   "cell_type": "markdown",
   "metadata": {
    "slideshow": {
     "slide_type": "fragment"
    }
   },
   "source": [
    "##### Solution:\n",
    "\n",
    "* Rewriting:\n",
    "\n",
    "\\begin{align}\n",
    "    f(x) & = \\frac{1}{x} \\\\\n",
    "    & = \\frac{1}{x + 1 - 1} \\\\\n",
    "    & = \\frac{1}{1 + x - 1} \\\\\n",
    "    & = \\frac{1}{1 + (x - 1)} \\\\\n",
    "    & = \\frac{1}{1 - (-x + 1)} \\\\\n",
    "    & = \\frac{1}{1 - (1 - x)} \\\\\n",
    "\\end{align}"
   ]
  },
  {
   "cell_type": "markdown",
   "metadata": {
    "slideshow": {
     "slide_type": "fragment"
    }
   },
   "source": [
    "* Then $f(x)$ can be represented as a geometric series with $a_0 = 1$ and $r = 1 - x$"
   ]
  },
  {
   "cell_type": "markdown",
   "metadata": {
    "slideshow": {
     "slide_type": "fragment"
    }
   },
   "source": [
    "* Therefore, we can express the function as a power series in the form\n",
    "\n",
    "\\begin{align}\n",
    "    f(x) & = \\sum_{k = 0}^\\infty \\left( 1 - x \\right)^k \\\\\n",
    "    & = \\sum_{k = 0}^\\infty \\left( -(x - 1) \\right)^k \\\\\n",
    "    & = \\sum_{k = 0}^\\infty (-1)^k \\left( x - 1 \\right)^k \\\\\n",
    "\\end{align}"
   ]
  },
  {
   "cell_type": "markdown",
   "metadata": {
    "slideshow": {
     "slide_type": "fragment"
    }
   },
   "source": [
    "* The interval of convergence is determined by $|r| = |x - 1| < 1$"
   ]
  },
  {
   "cell_type": "markdown",
   "metadata": {
    "slideshow": {
     "slide_type": "fragment"
    }
   },
   "source": [
    "* Therefore, the interval of convergence is\n",
    "\n",
    "\\begin{align}\n",
    "    & |x - 1| < 1 \\\\\n",
    "    & \\Rightarrow -1 < x - 1 < 1 \\\\\n",
    "    & \\Rightarrow 0 < x < 2 \\\\\n",
    "\\end{align}\n",
    "\n",
    "* Or in interval notation: $(0, 2)$"
   ]
  },
  {
   "cell_type": "markdown",
   "metadata": {
    "slideshow": {
     "slide_type": "slide"
    }
   },
   "source": [
    "##### Objective 2: Construct a power series using series operations"
   ]
  },
  {
   "cell_type": "markdown",
   "metadata": {
    "slideshow": {
     "slide_type": "fragment"
    }
   },
   "source": [
    "##### Operations with Power Series\n",
    "\n",
    "Let $\\displaystyle f(x) = \\sum_{k = 0}^\\infty a_k x^k$ and $\\displaystyle g(x) = \\sum_{k = 0}^\\infty b_k x^k$. Then for constants $h$ and $N$, the following properties hold.\n",
    "\n",
    "1. $\\displaystyle f(h x) = \\sum_{k = 0}^\\infty a_k h^k x^k$\n",
    "\n",
    "2. $\\displaystyle f(x^N) = \\sum_{k = 0}^\\infty a_k x^{kN}$\n",
    "\n",
    "3. $\\displaystyle f(x) \\pm g(x) = \\sum_{k = 0}^\\infty (a_k \\pm b_k) x^k$\n",
    "\n",
    "**Important Note:** Performing these operations may change the interval of convergence of the series that results!"
   ]
  },
  {
   "cell_type": "markdown",
   "metadata": {
    "slideshow": {
     "slide_type": "fragment"
    }
   },
   "source": [
    "##### Example 3\n",
    "\n",
    "Find a power series for $f(x) = \\frac{3x - 1}{x^2 - 1}$ centered at $c = 0$."
   ]
  },
  {
   "cell_type": "markdown",
   "metadata": {
    "slideshow": {
     "slide_type": "fragment"
    }
   },
   "source": [
    "##### Solution:\n",
    "\n",
    "* General approach: factor the denominator and perform partial fraction decomposition"
   ]
  },
  {
   "cell_type": "markdown",
   "metadata": {
    "slideshow": {
     "slide_type": "fragment"
    }
   },
   "source": [
    "* Factoring:\n",
    "\n",
    "\\begin{align}\n",
    "    f(x) & = \\frac{3x - 1}{(x + 1)(x - 1)}\n",
    "\\end{align}"
   ]
  },
  {
   "cell_type": "markdown",
   "metadata": {
    "slideshow": {
     "slide_type": "fragment"
    }
   },
   "source": [
    "* Partial fraction decomposition is performed below:\n",
    "\n",
    "\\begin{align}\n",
    "    f(x) = \\frac{3x - 1}{(x + 1)(x - 1)} & = \\frac{A}{x + 1} + \\frac{B}{x - 1}\n",
    "\\end{align}"
   ]
  },
  {
   "cell_type": "markdown",
   "metadata": {
    "slideshow": {
     "slide_type": "fragment"
    }
   },
   "source": [
    "* Mulitplying both sides by the common denominator $(x + 1)(x - 1)$:\n",
    "\n",
    "\\begin{align}\n",
    "    \\frac{3x - 1}{(x + 1)(x - 1)} \\cdot (x + 1)(x - 1) & = \\left( \\frac{A}{x + 1} + \\frac{B}{x - 1} \\right) (x + 1)(x - 1)\n",
    "\\end{align}"
   ]
  },
  {
   "cell_type": "markdown",
   "metadata": {
    "slideshow": {
     "slide_type": "fragment"
    }
   },
   "source": [
    "* Simplifying the left-hand side and distributing on the right-hand side:\n",
    "\n",
    "\\begin{align}\n",
    "    3x - 1 & = \\frac{A}{x + 1} \\cdot (x + 1)(x - 1) + \\frac{B}{x - 1} \\cdot (x + 1)(x - 1)\n",
    "\\end{align}"
   ]
  },
  {
   "cell_type": "markdown",
   "metadata": {
    "slideshow": {
     "slide_type": "fragment"
    }
   },
   "source": [
    "* Simplifying:\n",
    "\n",
    "\\begin{align}\n",
    "    3x - 1 & = A (x - 1) + B (x + 1)\n",
    "\\end{align}"
   ]
  },
  {
   "cell_type": "markdown",
   "metadata": {
    "slideshow": {
     "slide_type": "fragment"
    }
   },
   "source": [
    "* If $x = 1$, then\n",
    "\n",
    "\\begin{align}\n",
    "    3(1) - 1 & = A(1 - 1) + B(1 + 1) \\\\\n",
    "    2 & = 2B \\\\\n",
    "    B & = 1\n",
    "\\end{align}"
   ]
  },
  {
   "cell_type": "markdown",
   "metadata": {
    "slideshow": {
     "slide_type": "fragment"
    }
   },
   "source": [
    "* If $x = -1$, then\n",
    "\n",
    "\\begin{align}\n",
    "    3(-1) - 1 & = A (-1 - 1) + B (-1 + 1) \\\\\n",
    "    -4 & = -2A \\\\\n",
    "    A & = 2\n",
    "\\end{align}"
   ]
  },
  {
   "cell_type": "markdown",
   "metadata": {
    "slideshow": {
     "slide_type": "fragment"
    }
   },
   "source": [
    "* Therefore,\n",
    "\n",
    "\\begin{align}\n",
    "    f(x) & = \\frac{3x - 1}{x^2 - 1} \\\\\n",
    "    & = \\frac{2}{x + 1} + \\frac{1}{x - 1}\n",
    "\\end{align}"
   ]
  },
  {
   "cell_type": "markdown",
   "metadata": {
    "slideshow": {
     "slide_type": "fragment"
    }
   },
   "source": [
    "* Now we need to rewrite each fraction as a power series and add the two:\n",
    "\n",
    "* For $\\frac{2}{x + 1}$:\n",
    "\n",
    "\\begin{align}\n",
    "    \\frac{2}{x + 1} & = \\frac{2}{1 + x} \\\\\n",
    "    & = \\frac{2}{1 - (-x)}\n",
    "\\end{align}"
   ]
  },
  {
   "cell_type": "markdown",
   "metadata": {
    "slideshow": {
     "slide_type": "fragment"
    }
   },
   "source": [
    "* This can be expresses as a geometric series with $a_0 = 2$ and $r = -x$\n",
    "\n",
    "\\begin{align}\n",
    "    \\sum_{k = 0}^\\infty 2 (-x)^k & = \\sum_{k = 0}^\\infty 2 (-1)^k x^k\n",
    "\\end{align}\n",
    "\n",
    "* The above series has interval of convergence $|r| = |-x| = |x| < 1 \\Rightarrow -1 < x < 1$"
   ]
  },
  {
   "cell_type": "markdown",
   "metadata": {
    "slideshow": {
     "slide_type": "fragment"
    }
   },
   "source": [
    "* For $\\frac{1}{x - 1}$:\n",
    "\n",
    "\\begin{align}\n",
    "    \\frac{1}{x - 1} & = \\frac{1}{-1 + x} \\\\\n",
    "    & \\frac{1}{-(1 - x)} \\\\\n",
    "    & = \\frac{-1}{1 - x}\n",
    "\\end{align}"
   ]
  },
  {
   "cell_type": "markdown",
   "metadata": {
    "slideshow": {
     "slide_type": "fragment"
    }
   },
   "source": [
    "* This can be expressed as a geometric series with $a_0 = -1$ and $r = x$\n",
    "\n",
    "\\begin{align}\n",
    "    \\sum_{k = 0}^\\infty -x^k & = - \\sum_{k = 0}^\\infty x^k\n",
    "\\end{align}\n",
    "\n",
    "* The above series has interval of convergence $|r| = |x| < 1 \\Rightarrow -1 < x < 1$"
   ]
  },
  {
   "cell_type": "markdown",
   "metadata": {
    "slideshow": {
     "slide_type": "fragment"
    }
   },
   "source": [
    "* Therefore,\n",
    "\n",
    "\\begin{align}\n",
    "    f(x) & = \\sum_{k = 0}^\\infty 2 (-1)^k x^k - \\sum_{k = 0}^\\infty x^k \\\\\n",
    "    & = \\sum_{k = 0}^\\infty \\left( 2 (-1)^k x^k - x^k \\right) \\\\\n",
    "    & = \\sum_{k = 0}^\\infty \\left( 2 (-1)^k - 1 \\right) x^k \\\\\n",
    "\\end{align}"
   ]
  },
  {
   "cell_type": "markdown",
   "metadata": {
    "slideshow": {
     "slide_type": "fragment"
    }
   },
   "source": [
    "* The interval of convergence for this series is $(-1, 1)$"
   ]
  },
  {
   "cell_type": "markdown",
   "metadata": {
    "slideshow": {
     "slide_type": "fragment"
    }
   },
   "source": [
    "##### Example 4\n",
    "\n",
    "Find a power series for $f(x) = \\ln x$ centered at $c = 1$."
   ]
  },
  {
   "cell_type": "markdown",
   "metadata": {
    "slideshow": {
     "slide_type": "fragment"
    }
   },
   "source": [
    "##### Solution:\n",
    "\n",
    "* From example 2 we know that\n",
    "\n",
    "\\begin{align}\n",
    "    g(x) = \\frac{1}{x} = \\sum_{k = 0}^\\infty (-1)^k (x - 1)^k\n",
    "\\end{align}"
   ]
  },
  {
   "cell_type": "markdown",
   "metadata": {
    "slideshow": {
     "slide_type": "fragment"
    }
   },
   "source": [
    "* We also know that\n",
    "\n",
    "\\begin{align}\n",
    "    \\int \\frac{1}{x} \\, dx = \\ln x + C_1\n",
    "\\end{align}\n",
    "\n",
    "for some constant of integration $C_1$"
   ]
  },
  {
   "cell_type": "markdown",
   "metadata": {
    "slideshow": {
     "slide_type": "fragment"
    }
   },
   "source": [
    "* Therefore,\n",
    "\n",
    "\\begin{align}\n",
    "    \\ln x & = C_2 + \\int \\frac{1}{x} \\, dx \\\\\n",
    "    & = C_2 + \\int \\sum_{k = 0}^\\infty (-1)^k (x - 1)^k \\, dx \\\\\n",
    "    & = C_2 + \\sum_{k = 0}^\\infty (-1)^k \\int (x - 1)^k \\, dx \\\\\n",
    "    & = C + \\sum_{k = 0}^\\infty (-1)^k \\frac{(x - 1)^{k + 1}}{k + 1} \\\\\n",
    "\\end{align}"
   ]
  },
  {
   "cell_type": "markdown",
   "metadata": {
    "slideshow": {
     "slide_type": "fragment"
    }
   },
   "source": [
    "* If $x = 1$, then\n",
    "\n",
    "\\begin{align}\n",
    "    \\ln (1) & = 0 = C + 0 \\Rightarrow C = 0\n",
    "\\end{align}"
   ]
  },
  {
   "cell_type": "markdown",
   "metadata": {
    "slideshow": {
     "slide_type": "fragment"
    }
   },
   "source": [
    "* Therefore,\n",
    "\n",
    "\\begin{align}\n",
    "    \\ln x & = \\sum_{k = 0}^\\infty (-1)^k \\frac{(x - 1)^{k + 1}}{k + 1}\n",
    "\\end{align}"
   ]
  },
  {
   "cell_type": "markdown",
   "metadata": {
    "slideshow": {
     "slide_type": "fragment"
    }
   },
   "source": [
    "* To determine the interval of convergence we need apply the Ratio Test by letting $u_k = (-1)^k \\frac{(x - 1)^{k + 1}}{k + 1} \\Rightarrow u_{k + 1} = (-1)^{k + 1} \\frac{(x - 1)^{k + 2}}{k + 2}$"
   ]
  },
  {
   "cell_type": "markdown",
   "metadata": {
    "slideshow": {
     "slide_type": "fragment"
    }
   },
   "source": [
    "* The Ratio Test gives us\n",
    "\n",
    "\\begin{align}\n",
    "    \\lim_{k \\rightarrow \\infty} \\left| \\frac{u_{k + 1}}{u_k} \\right| & = \\lim_{k \\rightarrow \\infty} \\left| \\frac{(-1)^{k + 1} \\frac{(x - 1)^{k + 2}}{k + 2}}{(-1)^k \\frac{(x - 1)^{k + 1}}{k + 1}} \\right| \\\\\n",
    "    & = \\lim_{k \\rightarrow \\infty} \\left| \\frac{\\frac{(x - 1)^{k + 2}}{k + 2}}{\\frac{(x - 1)^{k + 1}}{k + 1}} \\right| \\\\\n",
    "    & = \\lim_{k \\rightarrow \\infty} \\left| \\frac{(x - 1)^{k + 2}}{k + 2} \\cdot \\frac{k + 1}{(x - 1)^{k + 1}} \\right| \\\\\n",
    "    & = \\lim_{k \\rightarrow \\infty} \\left| \\frac{k + 1}{k + 2} \\cdot \\frac{(x - 1)(x - 1)^{k + 1}}{(x - 1)^{k + 1}} \\right| \\\\\n",
    "    & = \\lim_{k \\rightarrow \\infty} \\left| \\frac{k + 1}{k + 2} \\cdot (x - 1) \\right| \\\\\n",
    "    & = \\lim_{k \\rightarrow \\infty} \\frac{k + 1}{k + 2} \\cdot \\left| x - 1 \\right| \\\\\n",
    "    & = \\left| x - 1 \\right| \\lim_{k \\rightarrow \\infty} \\frac{k + 1}{k + 2} \\\\\n",
    "    & = \\left| x - 1 \\right| \\cdot 1 \\\\\n",
    "    & = \\left| x - 1 \\right|\n",
    "\\end{align}"
   ]
  },
  {
   "cell_type": "markdown",
   "metadata": {
    "slideshow": {
     "slide_type": "fragment"
    }
   },
   "source": [
    "* For the Ratio Test to determine convergence we require $|x - 1| < 1$:\n",
    "\n",
    "\\begin{align}\n",
    "    & |x - 1| < 1 \\\\\n",
    "    & \\Rightarrow -1 < x - 1 < 1 \\\\\n",
    "    & \\Rightarrow 0 < x < 2\n",
    "\\end{align}"
   ]
  },
  {
   "cell_type": "markdown",
   "metadata": {
    "slideshow": {
     "slide_type": "fragment"
    }
   },
   "source": [
    "* If $x = 0$, then\n",
    "\n",
    "\\begin{align}\n",
    "    \\sum_{k = 0}^\\infty (-1)^k \\frac{(0 - 1)^{k + 1}}{k + 1} & = \\sum_{k = 0}^\\infty (-1)^k \\frac{(- 1)^{k + 1}}{k + 1} \\\\\n",
    "    & = \\sum_{k = 0}^\\infty \\frac{(- 1)^{2k + 1}}{k + 1} \\\\\n",
    "    & = \\sum_{k = 0}^\\infty \\frac{- 1}{k + 1} \\qquad (\\text{$2k + 1$ is always odd}) \\\\\n",
    "    & = -\\sum_{k = 0}^\\infty \\frac{1}{k + 1}\n",
    "\\end{align}\n",
    "\n",
    "* The above series is a general harmonic series, which diverges (or you could apply whichever appropriate test)"
   ]
  },
  {
   "cell_type": "markdown",
   "metadata": {
    "slideshow": {
     "slide_type": "fragment"
    }
   },
   "source": [
    "* If $x = 2$, then\n",
    "\n",
    "\\begin{align}\n",
    "    \\sum_{k = 0}^\\infty (-1)^k \\frac{(2 - 1)^{k + 1}}{k + 1} & = \\sum_{k = 0}^\\infty (-1)^k \\frac{ 1^{k + 1}}{k + 1} \\\\\n",
    "    & = \\sum_{k = 0}^\\infty \\frac{(- 1)^k}{k + 1}\n",
    "\\end{align}\n",
    "\n",
    "* The above series converges by the Alternating Series Test:\n",
    "\n",
    "    * $\\displaystyle \\lim_{k \\rightarrow \\infty} \\frac{1}{k + 1} = 0$\n",
    "    \n",
    "    * $a_{k + 1} = \\frac{1}{k + 2} \\leq \\frac{1}{k + 1} = a_k$"
   ]
  },
  {
   "cell_type": "markdown",
   "metadata": {
    "slideshow": {
     "slide_type": "fragment"
    }
   },
   "source": [
    "* Therefore, the inteval of convergence for the series is $(0, 2]$"
   ]
  },
  {
   "cell_type": "markdown",
   "metadata": {
    "slideshow": {
     "slide_type": "fragment"
    }
   },
   "source": [
    "* To restate our findings: $\\displaystyle f(x) = \\ln x = \\sum_{k = 0}^\\infty (-1)^k \\frac{(x - 1)^{k + 1}}{k + 1}$ with interval of convergence $(0, 2]$"
   ]
  },
  {
   "cell_type": "markdown",
   "metadata": {
    "slideshow": {
     "slide_type": "slide"
    }
   },
   "source": [
    "##### End of Section"
   ]
  }
 ],
 "metadata": {
  "celltoolbar": "Slideshow",
  "kernelspec": {
   "display_name": "Python 3",
   "language": "python",
   "name": "python3"
  },
  "language_info": {
   "codemirror_mode": {
    "name": "ipython",
    "version": 3
   },
   "file_extension": ".py",
   "mimetype": "text/x-python",
   "name": "python",
   "nbconvert_exporter": "python",
   "pygments_lexer": "ipython3",
   "version": "3.7.6"
  },
  "rise": {
   "enable_chalkboard": true,
   "theme": "sky",
   "transition": "zoom",
   "width": "110%"
  }
 },
 "nbformat": 4,
 "nbformat_minor": 4
}
